src/Rewriter/PerfTesting/Core.v
@@ -91,8 +91,9 @@ Module Import UnsaturatedSolinas.
       limbwidth := limbwidth n s c;
       machine_wordsize : Z }.
 
-  Global Instance show_params : Show params
-    := fun _ p => ("{| n := " ++ show false n ++ "; s := " ++ show false s ++ "; c := " ++ show false c ++ "; idxs := " ++ show false idxs ++ "; machine_wordsize := " ++ show false machine_wordsize ++ "|}")%string.
+  Global Instance show_lvl_params : ShowLevel params
+    := fun p => neg_wrap_parens ("{| n := " ++ show_lvl n term_lvl ++ "; s := " ++ show_lvl s term_lvl ++ "; c := " ++ show_lvl c term_lvl ++ "; idxs := " ++ show_lvl idxs term_lvl ++ "; machine_wordsize := " ++ show_lvl machine_wordsize term_lvl ++ "|}")%string.
+  Global Instance show_params : Show params := show_lvl_params.
 
   Definition of_string (p : string) (bitwidth : Z) : list params
     := match parseZ_arith_to_taps p with
@@ -159,7 +160,7 @@ Module Import UnsaturatedSolinas.
                     (seq _ _ id id)
                     (List.map
                        (fun method
-                        => let make_descr := fun kind => ("Testing UnsaturatedSolinas " ++ prime ++ " (bitwidth = " ++ str_bitwidth ++ " ) (index = " ++ str_index ++ " ) (method = " ++ show false method ++ " ) (params = " ++ show false p ++ " ) " ++ kind ++ " with extraction " ++ extr_descr)%string in
+                        => let make_descr := fun kind => ("Testing UnsaturatedSolinas " ++ prime ++ " (bitwidth = " ++ str_bitwidth ++ " ) (index = " ++ str_index ++ " ) (method = " ++ show method ++ " ) (params = " ++ show p ++ " ) " ++ kind ++ " with extraction " ++ extr_descr)%string in
                            (seq _ _)
                              (fun _ => time _ (make_descr "PipelineFullToStringsOf") (fun _ => PipelineFullToStringsOf (p, method)))
                              (fun _
@@ -302,8 +303,9 @@ Module Import WordByWordMontgomery.
             | None => 0
             end }.
 
-  Global Instance show_params : Show params
-    := fun _ p => ("{| m := " ++ show false m ++ "; machine_wordsize := " ++ show false machine_wordsize ++ "|}")%string.
+  Global Instance show_lvl_params : ShowLevel params
+    := fun p => neg_wrap_parens ("{| m := " ++ show_lvl m term_lvl ++ "; machine_wordsize := " ++ show_lvl machine_wordsize term_lvl ++ "|}")%string.
+  Global Instance show_params : Show params := show_lvl_params.
 
   Definition of_string (p : string) (bitwidth : Z) : option params
     := match parseZ_arith_strict p with
@@ -367,7 +369,7 @@ Module Import WordByWordMontgomery.
                     (seq _ _ id id)
                     (List.map
                        (fun method
-                        => let make_descr := fun kind => ("Testing WordByWordMontgomery " ++ prime ++ " (bitwidth = " ++ str_bitwidth ++ " ) (method = " ++ show false method ++ " ) (params = " ++ show false p ++ " ) " ++ kind ++ " with extraction " ++ extr_descr)%string in
+                        => let make_descr := fun kind => ("Testing WordByWordMontgomery " ++ prime ++ " (bitwidth = " ++ str_bitwidth ++ " ) (method = " ++ show method ++ " ) (params = " ++ show p ++ " ) " ++ kind ++ " with extraction " ++ extr_descr)%string in
                            (seq _ _)
                              (fun _ => time _ (make_descr "PipelineFullToStringsOf") (fun _ => PipelineFullToStringsOf (p, method)))
                              (fun _
