src/Util/ErrorT/Show.v
@@ -6,30 +6,30 @@ Import ListNotations.
 Local Open Scope list_scope.
 Local Open Scope string_scope.
 
-Global Instance show_ErrorT {ErrT T} {show_ErrT : Show ErrT} {show_T : Show T}
-  : Show (@ErrorT ErrT T)
-  := fun with_parens v
-     => maybe_wrap_parens
-          with_parens
-          match v with
-          | Success v => "Success " ++ show true v
-          | Error msg => "Error " ++ show true msg
-          end.
+Global Instance show_lvl_ErrorT {ErrT T} {show_ErrT : ShowLevel ErrT} {show_T : ShowLevel T}
+  : ShowLevel (@ErrorT ErrT T)
+  := fun v
+     => match v with
+        | Success v => show_lvl_app (fun 'tt => "Success") v
+        | Error msg => show_lvl_app (fun 'tt => "Error") msg
+        end.
+Global Instance show_ErrorT {ErrT T} {show_ErrT : Show ErrT} {show_T : Show T} : Show (@ErrorT ErrT T)
+  := let __ := @ShowLevel_of_Show ErrT in
+     let __ := @ShowLevel_of_Show T in
+     _.
 
 Global Instance show_lines_ErrorT {ErrT T} {show_lines_ErrT : ShowLines ErrT} {show_lines_T : ShowLines T}
   : ShowLines (@ErrorT ErrT T)
-  := fun with_parens v
-     => maybe_wrap_parens_lines
-          with_parens
-          (let '(prefix, lines)
-               := match v with
-                  | Success v => ("Success", show_lines true v)
-                  | Error msg => ("Error", show_lines true msg)
-                  end in
-           match lines with
-           | [] => [prefix ++ " ()"]
-           | [line] => [prefix ++ " " ++ line]
-           | lines => (([prefix ++ " ("]%string)
-                         ++ (List.map (fun s => "  " ++ s)%string lines)
-                         ++ [")"])%list
-           end).
+  := fun v
+     => let '(prefix, lines)
+            := match v with
+               | Success v => ("Success", show_lines v)
+               | Error msg => ("Error", show_lines msg)
+               end in
+        match lines with
+        | [] => [prefix ++ " ()"]
+        | [line] => [prefix ++ " " ++ line]
+        | lines => (([prefix ++ " ("]%string)
+                      ++ (List.map (fun s => "  " ++ s)%string lines)
+                      ++ [")"])%list
+        end.
