src/Util/MSetPositive/Show.v
@@ -5,4 +5,5 @@ Require Import Crypto.Util.Strings.Show.
 Module Import ShowMSetPositive := ShowWSets PositiveSet.
 
 Global Instance show_PositiveSet : Show PositiveSet.t := _.
-Global Instance show_lines_PositiveSet : ShowLines PositiveSet.t := _.
+Global Instance show_lvl_PositiveSet : ShowLevel PositiveSet.t := _.
+Global Instance show_lines_PositiveSet : ShowLines PositiveSet.t := let __ := @ShowLines_of_Show PositiveSet.elt in _.
